Examples/UniswapV2Pair/GetReserves.lean
@@ -201,7 +201,8 @@ theorem getReservesReturn1Mem_size (r0 r1 : UInt256) :
   rw [toByteArray_write_eq _ _ _ (by rw [getReservesReturn0Mem_size])
       (by rw [getReservesReturn0Mem_size]; exact lt_usize _ (by norm_num)),
     ByteArray.size_append, ByteArray.size_append, getReservesReturn0Mem_size,
-    ByteArray_zeroes_size, toByteArray_size]
+    ByteArray_zeroes_size, 
+    toByteArray_size]
 
 theorem getReservesReturnMem_size (r0 r1 ts : UInt256) :
     (getReservesReturnMem r0 r1 ts).size = 224 := by
@@ -209,7 +210,8 @@ theorem getReservesReturnMem_size (r0 r1 ts : UInt256) :
   rw [toByteArray_write_eq _ _ _ (by rw [getReservesReturn1Mem_size])
       (by rw [getReservesReturn1Mem_size]; exact lt_usize _ (by norm_num)),
     ByteArray.size_append, ByteArray.size_append, getReservesReturn1Mem_size,
-    ByteArray_zeroes_size, toByteArray_size]
+    ByteArray_zeroes_size, 
+    toByteArray_size]
 
 theorem getReservesReturn0Mem_read64 (r0 : UInt256) :
     (getReservesReturn0Mem r0).readWithPadding 64 32 = UInt256.toByteArray ⟨128⟩ := by
@@ -218,7 +220,8 @@ theorem getReservesReturn0Mem_read64 (r0 : UInt256) :
       (by rw [solcFreePtrMem_size]; exact lt_usize _ (by norm_num))]
   rw [readWithPadding_eq_extract _ 64 (by
       rw [ByteArray.size_append, ByteArray.size_append, solcFreePtrMem_size,
-        ByteArray_zeroes_size, toByteArray_size]
+        ByteArray_zeroes_size, 
+        toByteArray_size]
       native_decide)]
   rw [extract_append_left _ _ _ _ (by
       rw [ByteArray.size_append, solcFreePtrMem_size, ByteArray_zeroes_size]
@@ -257,36 +260,34 @@ theorem getReservesReturnMem_read128_96 (r0 r1 ts : UInt256) :
       (by rw [getReservesReturn1Mem_size]; exact lt_usize _ (by norm_num))]
   rw [extract_append_span
       (getReservesReturn1Mem r0 r1 ++
-        ffi.ByteArray.zeroes (192 - (getReservesReturn1Mem r0 r1).size))
+        ffi.ByteArray.zeroes ((192 - (getReservesReturn1Mem r0 r1).size)))
       (UInt256.toByteArray ts) 128 (128 + 96) (by
         rw [ByteArray.size_append, getReservesReturn1Mem_size, ByteArray_zeroes_size]
         omega) (by
         rw [ByteArray.size_append, getReservesReturn1Mem_size, ByteArray_zeroes_size]
         omega)]
   rw [ByteArray.size_append, getReservesReturn1Mem_size, ByteArray_zeroes_size]
-  rw [show ffi.ByteArray.zeroes (192 - 192) = ByteArray.empty by
-      exact zeroes_zero (n := 0) (by rfl)]
+  rw [show ffi.ByteArray.zeroes (192 - 192) = ByteArray.empty from zeroes_zero rfl]
   simp
   unfold getReservesReturn1Mem
   rw [toByteArray_write_eq _ _ _ (by rw [getReservesReturn0Mem_size])
       (by rw [getReservesReturn0Mem_size]; exact lt_usize _ (by norm_num))]
   rw [extract_append_span
       (getReservesReturn0Mem r0 ++
-        ffi.ByteArray.zeroes (160 - (getReservesReturn0Mem r0).size))
+        ffi.ByteArray.zeroes ((160 - (getReservesReturn0Mem r0).size)))
       (UInt256.toByteArray r1) 128 192 (by
         rw [ByteArray.size_append, getReservesReturn0Mem_size, ByteArray_zeroes_size]
         omega) (by
         rw [ByteArray.size_append, getReservesReturn0Mem_size, ByteArray_zeroes_size]
         omega)]
   rw [ByteArray.size_append, getReservesReturn0Mem_size, ByteArray_zeroes_size]
-  rw [show ffi.ByteArray.zeroes (160 - 160) = ByteArray.empty by
-      exact zeroes_zero (n := 0) (by rfl)]
+  rw [show ffi.ByteArray.zeroes (160 - 160) = ByteArray.empty from zeroes_zero rfl]
   simp
   unfold getReservesReturn0Mem
   rw [toByteArray_write_eq _ _ _ (by rw [solcFreePtrMem_size]; omega)
       (by rw [solcFreePtrMem_size]; exact lt_usize _ (by norm_num))]
   rw [extract_append_right_window
-      (solcFreePtrMem ++ ffi.ByteArray.zeroes (128 - solcFreePtrMem.size))
+      (solcFreePtrMem ++ ffi.ByteArray.zeroes ((128 - solcFreePtrMem.size)))
       (UInt256.toByteArray r0) 128 160 (by
         rw [ByteArray.size_append, solcFreePtrMem_size, ByteArray_zeroes_size])]
   rw [ByteArray.size_append, solcFreePtrMem_size, ByteArray_zeroes_size]
