Examples/UniswapV2Pair/Routines.lean
@@ -1093,7 +1093,8 @@ theorem uniswapTransferLogMem_size (src toWord value : UInt256) :
   rw [toByteArray_write_eq _ _ _ (by rw [uniswapTransferCreditHashMem_size]; omega)
       (by rw [uniswapTransferCreditHashMem_size]; exact lt_usize _ (by norm_num)),
     ByteArray.size_append, ByteArray.size_append, uniswapTransferCreditHashMem_size,
-    ByteArray_zeroes_size, toByteArray_size]
+    ByteArray_zeroes_size,
+    toByteArray_size]
 
 theorem uniswapTransferLogMem_read64 (src toWord value : UInt256) :
     (uniswapTransferLogMem src toWord value).readWithPadding 64 32 =
@@ -1131,10 +1132,11 @@ theorem uniswapTransferLogMem_read128 (src toWord value : UInt256) :
       (by rw [uniswapTransferCreditHashMem_size]; exact lt_usize _ (by norm_num))]
   rw [readWithPadding_eq_extract _ 128 (by
       rw [ByteArray.size_append, ByteArray.size_append, uniswapTransferCreditHashMem_size,
-        ByteArray_zeroes_size, toByteArray_size])]
+        ByteArray_zeroes_size, 
+        toByteArray_size])]
   rw [extract_append_right_window
       (uniswapTransferCreditHashMem src toWord ++
-        ffi.ByteArray.zeroes (128 - (uniswapTransferCreditHashMem src toWord).size))
+        ffi.ByteArray.zeroes ((128 - (uniswapTransferCreditHashMem src toWord).size)))
       (UInt256.toByteArray value) 128 (128 + 32) (by
         rw [ByteArray.size_append, uniswapTransferCreditHashMem_size, ByteArray_zeroes_size])]
   rw [ByteArray.size_append, uniswapTransferCreditHashMem_size, ByteArray_zeroes_size]
@@ -1350,7 +1352,8 @@ theorem uniswapApproveLogMem_size (owner spender value : UInt256) :
   rw [toByteArray_write_eq _ _ _ (by rw [uniswapApproveHashMem_size]; omega)
       (by rw [uniswapApproveHashMem_size]; exact lt_usize _ (by norm_num)),
     ByteArray.size_append, ByteArray.size_append, uniswapApproveHashMem_size,
-    ByteArray_zeroes_size, toByteArray_size]
+    ByteArray_zeroes_size,
+    toByteArray_size]
 
 theorem uniswapApproveLogMem_read64 (owner spender value : UInt256) :
     (uniswapApproveLogMem owner spender value).readWithPadding 64 32 =
@@ -1388,10 +1391,11 @@ theorem uniswapApproveLogMem_read128 (owner spender value : UInt256) :
       (by rw [uniswapApproveHashMem_size]; exact lt_usize _ (by norm_num))]
   rw [readWithPadding_eq_extract _ 128 (by
       rw [ByteArray.size_append, ByteArray.size_append, uniswapApproveHashMem_size,
-        ByteArray_zeroes_size, toByteArray_size])]
+        ByteArray_zeroes_size, 
+        toByteArray_size])]
   rw [extract_append_right_window
       (uniswapApproveHashMem owner spender ++
-        ffi.ByteArray.zeroes (128 - (uniswapApproveHashMem owner spender).size))
+        ffi.ByteArray.zeroes ((128 - (uniswapApproveHashMem owner spender).size)))
       (UInt256.toByteArray value) 128 (128 + 32) (by
         rw [ByteArray.size_append, uniswapApproveHashMem_size, ByteArray_zeroes_size])]
   rw [ByteArray.size_append, uniswapApproveHashMem_size, ByteArray_zeroes_size]
